tla-tree/KVTypes.dfy
@@ -8,6 +8,9 @@ predicate KeyLeq(a:Key, b:Key) {
     KeyLe(a, b) || a==b
 }
 
+lemma KeyLeTransitive()
+    ensures forall a, b, c :: KeyLe(a,b) && KeyLe(b,c) ==> KeyLe(a,c)
+
 function MIN_KEY() : Key
     ensures forall k :: KeyLeq( MIN_KEY(), k)
 
